

Assignment 14

Find $f'(x)$

①

$$f(x) = (x^3 + x^2) \cdot (x^4 + x^5)$$

$$\begin{aligned} f'(x) &= (x^3 + x^2)' \cdot (x^4 + x^5) + (x^3 + x^2) \cdot (x^4 + x^5)' \\ &= (3x^2 + 2x)(x^4 + x^5) + (x^3 + x^2) \cdot (4x^3 + 5x^4) \end{aligned}$$

product

② $f(x) = (2x^4 + 6x + 1) \cdot (6x^4 + 3x^2 + 2024)$

$$\begin{aligned} f'(x) &= (2x^4 + 6x + 1)' \cdot (6x^4 + 3x^2 + 2024) + (2x^4 + 6x + 1) \cdot (6x^4 + 3x^2 + 2024)' \\ &= (8x^3 + 6) \cdot (6x^4 + 3x^2 + 2024) + (2x^4 + 6x + 1) \cdot (24x^3 + 6x) \end{aligned}$$

③ $f(x) = (\sqrt{x} + 1) \cdot (2x^3 + x + 1)$

$$f'(x) = (x^{1/2} + 1)' \cdot (2x^3 + x + 1) + (\sqrt{x} + 1) \cdot (2x^3 + x + 1)'$$

$$f'(x) = \frac{1}{2}x^{-1/2} \cdot (2x^3 + x + 1) + (\sqrt{x} + 1) \cdot (6x^2 + 1)$$

④ Do #1 not using the product rule.

$$f(x) = (x^3 + x^2) \cdot (x^4 + x^5)$$

$$f(x) = x^3 \cdot x^4 + x^3 \cdot x^5 + x^2 \cdot x^4 + x^2 \cdot x^5$$

$$f(x) = \underline{x^7} + x^8 + x^6 + \underline{x^7}$$

$$f(x) = x^8 + 2x^7 + x^6$$

$$f'(x) = 8x^7 + 14x^6 + 6x^5$$

Rule 6: Quotient Rule

$$\left[\frac{\text{top}}{\text{bot}} \right]' = \frac{(\text{top})' \cdot \text{bot} - \text{top} \cdot (\text{bot})'}{(\text{bot})^2}$$

Quotient

Example:

① $f(x) = \frac{3x+1}{7x+2}$

$$\Rightarrow f'(x) = \frac{(3x+1)' \cdot (7x+2) - (3x+1) \cdot (7x+2)'}{(7x+2)^2}$$

$$f'(x) = \frac{3 \cdot (7x+2) - (3x+1) \cdot 7}{(7x+2)^2} \quad (\text{done taking derivative})$$

$$f'(x) = \frac{21x + 6 - 21x - 7}{(7x+2)^2}$$

simplifying

$$f'(x) = \frac{-1}{(7x+2)^2}$$

② Find $f'(x)$ and simplify $f'(x)$

$$f(x) = \frac{x^2 + 2x}{x^2 + 7}$$

$$f'(x) = \frac{(x^2 + 2x)' \cdot (x^2 + 7) - (x^2 + 2x) \cdot (x^2 + 7)'}{(x^2 + 7)^2}$$

$$f'(x) = \frac{(2x + 2)(x^2 + 7) - (x^2 + 2x)(2x)}{(x^2 + 7)^2}$$

$$f'(x) = \frac{2x^3 + 14x + 2x^2 + 14 - 2x^3 - 4x^2}{(x^2 + 7)^2}$$

$$f'(x) = \frac{-2x^2 + 14x + 14}{(x^2 + 7)^2}$$

Assignment 15:

① Find $f'(x)$ (no need to simplify $f'(x)$)

① $f(x) = \frac{x^3 + x}{x^2 + 2x}$

② $f(x) = \frac{x^7 + x^6}{x^6 + 2x^5 + 2024}$

③ $f(x) = \frac{x^3 + 3}{x + 3}$

④ $f(x) = \frac{2x^6 + 2x}{2x^5 + 7}$

② Find $f'(x)$ and simplify $f'(x)$

① $f(x) = \frac{7x + 2}{6x + 9}$

② $f(x) = \frac{x^2 + 2}{x^2 + 3}$

③ $f(x) = \frac{x^3 + 1}{x^3 + 2}$

Rule 7: Exponential Rule

① $(b^x)' = b^x \cdot \ln b$

note: $\ln b = \log_e b$

$e = 2.71828...$

② $(e^x)' = e^x$

Example: Find $f'(x)$

$$① f(x) = 2^x \Rightarrow f'(x) = 2^x \cdot \ln 2$$

$$② f(x) = 3^x \Rightarrow f'(x) = 3^x \cdot \ln 3$$

$$③ f(x) = 2024^x \Rightarrow f'(x) = 2024^x \cdot \ln 2024$$

$$④ f(x) = \frac{e^x + 1}{e^x + 2}$$

$$\Rightarrow f'(x) = \frac{(e^x + 1)' \cdot (e^x + 2) - (e^x + 1) \cdot (e^x + 2)'}{(e^x + 2)^2}$$

$$f'(x) = \frac{e^x \cdot (e^x + 2) - e^x (e^x)}{(e^x + 2)^2}$$

$$f'(x) = \frac{e^x \cdot e^x + 2e^x - e^x \cdot e^x}{(e^x + 2)^2}$$

$$f'(x) = \frac{2e^x}{(e^x + 2)^2}$$

$$⑤ f(x) = x^2 \cdot 7^x$$

product

$$f'(x) = (x^2)' \cdot 7^x + x^2 \cdot (7^x)'$$

$$f'(x) = 2x \cdot 7^x + x^2 \cdot 7^x \cdot \ln 7$$

$$⑥ \quad f(x) = (3^x + 1) \cdot (x^2 + 3)$$

product

$$f'(x) = (3^x + 1)' \cdot (x^2 + 3) + (3^x + 1) \cdot (x^2 + 3)'$$

$$f'(x) = 3^x \cdot \ln 3 \cdot (x^2 + 3) + (3^x + 1) \cdot (2x)$$

Assignment 16

A. Find $f'(x)$. no need to simplify $f'(x)$.

$$① \quad f(x) = 3^x$$

$$② \quad f(x) = 20^x$$

$$③ \quad f(x) = (\sqrt{3})^x$$

$$④ \quad f(x) = 6^x + 7^x + 8^x$$

$$⑤ \quad f(x) = \underset{\substack{\uparrow \\ \text{scalar}}}{3} \cdot 9^x + \underset{\uparrow}{7} \cdot 6^x + \underset{\uparrow}{4} \cdot 2^x$$

Solution: $f'(x) = 3 \cdot 9^x \cdot \ln 9 + 7 \cdot 6^x \cdot \ln 6 + 4 \cdot 2^x \cdot \ln 2$

$$⑥ \quad f(x) = 4 \cdot 20^x - 7 \cdot 4^x + 16 \cdot 15^x + 1$$

$$⑦ \quad f(x) = (x^2 + 1) \cdot 11^x$$

$$⑧ \quad f(x) = (x + 9) \cdot (7^x + 6^x)$$

$$⑨ \quad f(x) = x \cdot e^x$$

$$⑩ \quad f(x) = \frac{x^2 + 2}{e^x}$$

$$(11) \quad f(x) = \frac{3^x + 2}{4^x + 1}$$

$$(12) \quad f(x) = \frac{x}{e^x}$$

B. Find and simplify $f'(x)$

$$(1) \quad f(x) = \frac{2^x + 1}{2^x + 9}$$

$$(2) \quad f(x) = \frac{e^x + x + 1}{e^x + x + 2}$$

C. For extra credit

$$f(x) = \frac{x \cdot e^x}{(x+1) \cdot 2^x}$$